kalloc/kalloc.v
@@ -81,7 +81,6 @@ Definition _client12 : ident := $"client12".
 Definition _client13 : ident := $"client13".
 Definition _client5 : ident := $"client5".
 Definition _client6 : ident := $"client6".
-Definition _client8 : ident := $"client8".
 Definition _client9 : ident := $"client9".
 Definition _data : ident := $"data".
 Definition _freelist : ident := $"freelist".
@@ -93,6 +92,7 @@ Definition _kalloc_write_42_kfree : ident := $"kalloc_write_42_kfree".
 Definition _kalloc_write_pipe : ident := $"kalloc_write_pipe".
 Definition _kfree : ident := $"kfree".
 Definition _kfree_kalloc : ident := $"kfree_kalloc".
+Definition _kfree_kalloc_kfree_kalloc : ident := $"kfree_kalloc_kfree_kalloc".
 Definition _kfree_kalloc_twice : ident := $"kfree_kalloc_twice".
 Definition _kmem : ident := $"kmem".
 Definition _main : ident := $"main".
@@ -317,6 +317,29 @@ Definition f_kfree_kalloc_twice := {|
     (Sreturn (Some (Etempvar _t'1 (tptr tvoid))))))
 |}.
 
+Definition f_kfree_kalloc_kfree_kalloc := {|
+  fn_return := (tptr tvoid);
+  fn_callconv := cc_default;
+  fn_params := ((_pa1, (tptr tvoid)) :: (_pa2, (tptr tvoid)) :: nil);
+  fn_vars := nil;
+  fn_temps := ((_t'1, (tptr tvoid)) :: nil);
+  fn_body :=
+(Ssequence
+  (Scall None
+    (Evar _kfree (Tfunction ((tptr tvoid) :: nil) tvoid cc_default))
+    ((Etempvar _pa1 (tptr tvoid)) :: nil))
+  (Ssequence
+    (Scall None (Evar _kalloc (Tfunction nil (tptr tvoid) cc_default)) nil)
+    (Ssequence
+      (Scall None
+        (Evar _kfree (Tfunction ((tptr tvoid) :: nil) tvoid cc_default))
+        ((Etempvar _pa2 (tptr tvoid)) :: nil))
+      (Ssequence
+        (Scall (Some _t'1)
+          (Evar _kalloc (Tfunction nil (tptr tvoid) cc_default)) nil)
+        (Sreturn (Some (Etempvar _t'1 (tptr tvoid))))))))
+|}.
+
 Definition f_freerange_while_loop := {|
   fn_return := tvoid;
   fn_callconv := cc_default;
@@ -380,29 +403,6 @@ Definition f_client6 := {|
       (Scall (Some _t'1)
         (Evar _kalloc (Tfunction nil (tptr tvoid) cc_default)) nil)
       (Sreturn (Some (Etempvar _t'1 (tptr tvoid)))))))
-|}.
-
-Definition f_client8 := {|
-  fn_return := (tptr tvoid);
-  fn_callconv := cc_default;
-  fn_params := ((_pa1, (tptr tvoid)) :: (_pa2, (tptr tvoid)) :: nil);
-  fn_vars := nil;
-  fn_temps := ((_t'1, (tptr tvoid)) :: nil);
-  fn_body :=
-(Ssequence
-  (Scall None
-    (Evar _kfree (Tfunction ((tptr tvoid) :: nil) tvoid cc_default))
-    ((Etempvar _pa1 (tptr tvoid)) :: nil))
-  (Ssequence
-    (Scall None (Evar _kalloc (Tfunction nil (tptr tvoid) cc_default)) nil)
-    (Ssequence
-      (Scall None
-        (Evar _kfree (Tfunction ((tptr tvoid) :: nil) tvoid cc_default))
-        ((Etempvar _pa2 (tptr tvoid)) :: nil))
-      (Ssequence
-        (Scall (Some _t'1)
-          (Evar _kalloc (Tfunction nil (tptr tvoid) cc_default)) nil)
-        (Sreturn (Some (Etempvar _t'1 (tptr tvoid))))))))
 |}.
 
 Definition f_client9 := {|
@@ -796,10 +796,10 @@ Definition global_definitions : list (ident * globdef fundef type) :=
  (_kalloc_write_42_kfree, Gfun(Internal f_kalloc_write_42_kfree)) ::
  (_kalloc_write_pipe, Gfun(Internal f_kalloc_write_pipe)) ::
  (_kfree_kalloc_twice, Gfun(Internal f_kfree_kalloc_twice)) ::
+ (_kfree_kalloc_kfree_kalloc, Gfun(Internal f_kfree_kalloc_kfree_kalloc)) ::
  (_freerange_while_loop, Gfun(Internal f_freerange_while_loop)) ::
  (_client5, Gfun(Internal f_client5)) ::
  (_client6, Gfun(Internal f_client6)) ::
- (_client8, Gfun(Internal f_client8)) ::
  (_client9, Gfun(Internal f_client9)) ::
  (_client10, Gfun(Internal f_client10)) ::
  (_client11, Gfun(Internal f_client11)) ::
@@ -807,29 +807,30 @@ Definition global_definitions : list (ident * globdef fundef type) :=
  (_client13, Gfun(Internal f_client13)) :: nil).
 
 Definition public_idents : list ident :=
-(_client13 :: _client12 :: _client11 :: _client10 :: _client9 :: _client8 ::
- _client6 :: _client5 :: _freerange_while_loop :: _kfree_kalloc_twice ::
- _kalloc_write_pipe :: _kalloc_write_42_kfree :: _kalloc_write_42 ::
- _kfree_kalloc :: _kalloc :: _kfree :: _kmem :: ___builtin_debug ::
- ___builtin_write32_reversed :: ___builtin_write16_reversed ::
- ___builtin_read32_reversed :: ___builtin_read16_reversed ::
- ___builtin_fnmsub :: ___builtin_fnmadd :: ___builtin_fmsub ::
- ___builtin_fmadd :: ___builtin_fmin :: ___builtin_fmax ::
- ___builtin_expect :: ___builtin_unreachable :: ___builtin_va_end ::
- ___builtin_va_copy :: ___builtin_va_arg :: ___builtin_va_start ::
- ___builtin_membar :: ___builtin_annot_intval :: ___builtin_annot ::
- ___builtin_sel :: ___builtin_memcpy_aligned :: ___builtin_sqrt ::
- ___builtin_fsqrt :: ___builtin_fabsf :: ___builtin_fabs ::
- ___builtin_ctzll :: ___builtin_ctzl :: ___builtin_ctz :: ___builtin_clzll ::
- ___builtin_clzl :: ___builtin_clz :: ___builtin_bswap16 ::
- ___builtin_bswap32 :: ___builtin_bswap :: ___builtin_bswap64 ::
- ___compcert_i64_umulh :: ___compcert_i64_smulh :: ___compcert_i64_sar ::
- ___compcert_i64_shr :: ___compcert_i64_shl :: ___compcert_i64_umod ::
- ___compcert_i64_smod :: ___compcert_i64_udiv :: ___compcert_i64_sdiv ::
- ___compcert_i64_utof :: ___compcert_i64_stof :: ___compcert_i64_utod ::
- ___compcert_i64_stod :: ___compcert_i64_dtou :: ___compcert_i64_dtos ::
- ___compcert_va_composite :: ___compcert_va_float64 ::
- ___compcert_va_int64 :: ___compcert_va_int32 :: nil).
+(_client13 :: _client12 :: _client11 :: _client10 :: _client9 :: _client6 ::
+ _client5 :: _freerange_while_loop :: _kfree_kalloc_kfree_kalloc ::
+ _kfree_kalloc_twice :: _kalloc_write_pipe :: _kalloc_write_42_kfree ::
+ _kalloc_write_42 :: _kfree_kalloc :: _kalloc :: _kfree :: _kmem ::
+ ___builtin_debug :: ___builtin_write32_reversed ::
+ ___builtin_write16_reversed :: ___builtin_read32_reversed ::
+ ___builtin_read16_reversed :: ___builtin_fnmsub :: ___builtin_fnmadd ::
+ ___builtin_fmsub :: ___builtin_fmadd :: ___builtin_fmin ::
+ ___builtin_fmax :: ___builtin_expect :: ___builtin_unreachable ::
+ ___builtin_va_end :: ___builtin_va_copy :: ___builtin_va_arg ::
+ ___builtin_va_start :: ___builtin_membar :: ___builtin_annot_intval ::
+ ___builtin_annot :: ___builtin_sel :: ___builtin_memcpy_aligned ::
+ ___builtin_sqrt :: ___builtin_fsqrt :: ___builtin_fabsf ::
+ ___builtin_fabs :: ___builtin_ctzll :: ___builtin_ctzl :: ___builtin_ctz ::
+ ___builtin_clzll :: ___builtin_clzl :: ___builtin_clz ::
+ ___builtin_bswap16 :: ___builtin_bswap32 :: ___builtin_bswap ::
+ ___builtin_bswap64 :: ___compcert_i64_umulh :: ___compcert_i64_smulh ::
+ ___compcert_i64_sar :: ___compcert_i64_shr :: ___compcert_i64_shl ::
+ ___compcert_i64_umod :: ___compcert_i64_smod :: ___compcert_i64_udiv ::
+ ___compcert_i64_sdiv :: ___compcert_i64_utof :: ___compcert_i64_stof ::
+ ___compcert_i64_utod :: ___compcert_i64_stod :: ___compcert_i64_dtou ::
+ ___compcert_i64_dtos :: ___compcert_va_composite ::
+ ___compcert_va_float64 :: ___compcert_va_int64 :: ___compcert_va_int32 ::
+ nil).
 
 Definition prog : Clight.program := 
   mkprogram composites global_definitions public_idents _main Logic.I.
